{"nbformat":4,"nbformat_minor":0,"metadata":{"colab":{"provenance":[],"authorship_tag":"ABX9TyOlrqdBGhdk6Ot1NLgwh/Mt"},"kernelspec":{"name":"python3","display_name":"Python 3"},"language_info":{"name":"python"}},"cells":[{"cell_type":"code","source":["# All we need for functional programming in Python\n","import functools\n","import operator"],"metadata":{"id":"l56mSqA9W-_8","executionInfo":{"status":"ok","timestamp":1750190936424,"user_tz":240,"elapsed":5,"user":{"displayName":"Peter Fackeldey","userId":"16959509108257278929"}}},"execution_count":1,"outputs":[]},{"cell_type":"code","execution_count":2,"metadata":{"colab":{"base_uri":"https://localhost:8080/"},"id":"xlSC5LJxWlUU","executionInfo":{"status":"ok","timestamp":1750190936493,"user_tz":240,"elapsed":57,"user":{"displayName":"Peter Fackeldey","userId":"16959509108257278929"}},"outputId":"577601f4-7948-45db-ec8b-376854593a3d"},"outputs":[{"output_type":"stream","name":"stdout","text":["1 + 2 = 3\n","10 (+ 3) (+ 3) = 16\n","Hip Hip Hurray!\n"]}],"source":["# Currying\n","\n","# Currying Haskell example to add 1\n","# ```haskell\n","#   let addOne = (+ 1)\n","#   putStrLn $ \"1 + 2 = \" ++ show (addOne 2)\n","#   >> 1 + 2 = 3\n","# ```\n","#\n","# Python equivalent:\n","# - functools.partial: allows currying\n","# - operator.add: is the addition function\n","addOne = functools.partial(operator.add, 1)\n","print(\"1 + 2 =\", addOne(2))\n","\n","# Currying Haskell example to add a function twice\n","# ```haskell\n","#   let applyFnTwice f x = f (f x)\n","#   let addThreeTwice = applyFnTwice (+ 3)\n","#   putStrLn $ \"10 (+ 3) (+ 3) = \" ++ show (addThreeTwice 10)\n","#   >> 10 (+ 3) (+ 3) = 16\n","# ```\n","#\n","# Python equivalent:\n","def applyFnTwice(f, x):\n","  return f(f(x))\n","\n","addThree = functools.partial(operator.add, 3)\n","addThreeTwice = functools.partial(applyFnTwice, addThree)\n","\n","print(\"10 (+ 3) (+ 3) =\", addThreeTwice(10))\n","\n","# Another applyFnTwice example\n","# ```haskell\n","#   let hipHip = applyFnTwice (\"Hip \" ++)\n","#   putStrLn $ hipHip \"Hurray!\"\n","#   >> Hip Hip Hurray!\n","# ```\n","#\n","# Python equivalent:\n","hipHip = functools.partial(applyFnTwice, \"Hip {}\".format)\n","print(hipHip(\"Hurray!\"))"]},{"cell_type":"code","source":["# Recursion\n","values = [2, 1, 5, 3, 4]\n","\n","# Recursion Haskell example for `sum`\n","# ```haskell\n","#   let sum' :: (Num a) => [a] -> a\n","#       sum' [] = 0\n","#       sum' (x : xs) = x + sum' xs\n","#   putStrLn $ \"Summing \" ++ show values ++ \": \" ++ show (sum' values)\n","#   >> Summing [2,1,5,3,4]: 15\n","# ```\n","#\n","# Python equivalent:\n","def sum_(vals):\n","  # empty list case\n","  if not vals:\n","    return 0\n","  # recurse\n","  return vals[0] + sum_(vals[1:])\n","\n","print(f\"Summing {values} :\", sum_(values))\n","\n","\n","# Recursion Haskell example for Fibonacci sequence\n","# ```haskell\n","#   let fib :: Int -> Int\n","#       fib 0 = 1\n","#       fib 1 = 1\n","#       fib n = fib (n - 1) + fib (n - 2)\n","#   putStrLn $ \"Fibonacci(12) = \" ++ show (fib 12)\n","#   >> Fibonacci(12) = 233\n","# ```\n","#\n","# Python equivalent:\n","def fib(n):\n","  # edge case conditions\n","  if n == 0 or n == 1:\n","    return 1\n","  # recurse\n","  return fib (n - 1) + fib (n - 2)\n","\n","print(\"Fibonacci(12) =\", fib(12))\n","\n","\n","# Recursion Haskell example for `map`\n","# ```haskell\n","#   let map' :: (a -> b) -> [a] -> [b]\n","#       map' _ [] = []\n","#       map' f (x : xs) = f x : map' f xs\n","#\n","#   let addOneToEach = map' addOne\n","#   putStrLn $ \"Increase each value from \" ++ show values ++ \" by 1: \" ++ show (addOneToEach values)\n","#   >> Increase each value from [2,1,5,3,4] by 1: [3,2,6,4,5]\n","# ```\n","#\n","# Python equivalent:\n","def map_(f, xs):\n","  # empty list case\n","  if not xs:\n","    return []\n","  # first element: [f(xs[0])]\n","  # recurse through remaining ones: map_(f, xs[1:])\n","  return [f(xs[0])] + map_(f, xs[1:])\n","\n","addOneToEach = functools.partial(map_, addOne)\n","print(f\"Increase each value from {values} by 1:\", addOneToEach(values))\n","\n","\n","# Recursion Haskell example for `filter`\n","# ```haskell\n","#   let filter' :: (a -> Bool) -> [a] -> [a]\n","#       filter' _ [] = []\n","#       filter' p (x : xs)\n","#         | p x = x : filter' p xs\n","#         | otherwise = filter' p xs\n","#\n","#   let selectEqThree = filter' (== 3)\n","#   let values = [2, 1, 5, 3, 4]\n","#   putStrLn $ \"Select only the 3 from \" ++ show values ++ \": \" ++ show (selectEqThree values)\n","#   >> Select only the 3 from [2,1,5,3,4]: [3]\n","# ```\n","#\n","# Python equivalent:\n","def filter_(p, xs):\n","  # empty list case\n","  if not xs:\n","    return []\n","  # recurse through `xs`, keep `xs[0]` if p(xs[0]) == True\n","  return ([xs[0]] if p(xs[0]) else []) + filter_(p, xs[1:])\n","\n","\n","# double-currying\n","selectEqThree = functools.partial(filter_, functools.partial(operator.eq, 3))\n","print(f\"Select only the 3 from {values}:\", selectEqThree(values))\n","\n","\n","# Recursion Haskell example for quicksort:\n","# ```haskell\n","#   let quicksort :: (Ord a) => [a] -> [a]\n","#       quicksort [] = []\n","#       quicksort (x : xs) =\n","#         let smallerSorted = quicksort (filter (<= x) xs)\n","#             biggerSorted = quicksort (filter (> x) xs)\n","#          in smallerSorted ++ [x] ++ biggerSorted\n","#\n","#   let sortedValues = quicksort values\n","#   putStrLn $ \"Sorting \" ++ show values ++ \" results in \" ++ show sortedValues\n","#   >> Sorting [2,1,5,3,4] results in [1,2,3,4,5]\n","# ```\n","#\n","# Python equivalent:\n","def quicksort(xs):\n","  # empty list case\n","  if not xs:\n","    return []\n","  # recurse\n","  smallerSorted = quicksort(filter_(functools.partial(operator.ge, xs[0]), xs[1:]))\n","  biggerSorted = quicksort(filter_(functools.partial(operator.lt, xs[0]), xs[1:]))\n","  return smallerSorted + [xs[0]] + biggerSorted\n","\n","\n","print(f\"Sorting {values} results in\", quicksort(values))"],"metadata":{"colab":{"base_uri":"https://localhost:8080/"},"id":"ancJ6tVIY0Yr","executionInfo":{"status":"ok","timestamp":1750190936494,"user_tz":240,"elapsed":6,"user":{"displayName":"Peter Fackeldey","userId":"16959509108257278929"}},"outputId":"23a7e19f-9f8b-4a56-a83d-05a3d1fa601c"},"execution_count":3,"outputs":[{"output_type":"stream","name":"stdout","text":["Summing [2, 1, 5, 3, 4] : 15\n","Fibonacci(12) = 233\n","Increase each value from [2, 1, 5, 3, 4] by 1: [3, 2, 6, 4, 5]\n","Select only the 3 from [2, 1, 5, 3, 4]: [3]\n","Sorting [2, 1, 5, 3, 4] results in [1, 2, 3, 4, 5]\n"]}]},{"cell_type":"code","source":["# Lambdas:\n","listOfTuples = [(1, 1), (2, 2), (3, 3), (4, 4), (5, 5)]\n","\n","# Lambda Haskell example for summing all tuples inside a list\n","# ```haskell\n","#   let sumAllTuples = map' (\\(a, b) -> (+ a) b)\n","#   putStrLn $ \"Summing up all tuples inside \" ++ show listOfTuples ++ \" yields: \" ++ show (sumAllTuples listOfTuples)\n","#   >> Summing up all tuples inside [(1,1),(2,2),(3,3),(4,4),(5,5)] yields: [2,4,6,8,10]\n","# ```\n","#\n","# Python equivalent:\n","sumAllTuples = functools.partial(map_, lambda x: x[0] + x[1])\n","print(f\"Summing up all tuples inside {listOfTuples} yields:\", sumAllTuples(listOfTuples))\n","\n","# Lambda Haskell example for flipping the arguments of a function `f`\n","# ```haskell\n","#   let flip' :: (a -> b -> c) -> b -> a -> c\n","#       flip' f = \\x y -> f y x\n","#\n","#   let flipped_substraction = flip' (-)\n","#   putStrLn $ \"Flipping `3-1` to `1-3`: \" ++ show (flipped_substraction 3 1)\n","#   >> Flipping `3-1` to `1-3`: -2\n","# ```\n","#\n","# Python equivalent:\n","def flip(f):\n","  return lambda x,y: f(y, x)\n","\n","flipped_substraction = flip(operator.sub)\n","print(\"Flipping `3-1` to `1-3`:\", flipped_substraction(3, 1))"],"metadata":{"colab":{"base_uri":"https://localhost:8080/"},"id":"SGKDi8c5eYTF","executionInfo":{"status":"ok","timestamp":1750190936496,"user_tz":240,"elapsed":4,"user":{"displayName":"Peter Fackeldey","userId":"16959509108257278929"}},"outputId":"525ea6e4-a014-4e1a-bb65-5337ccd9e477"},"execution_count":4,"outputs":[{"output_type":"stream","name":"stdout","text":["Summing up all tuples inside [(1, 1), (2, 2), (3, 3), (4, 4), (5, 5)] yields: [2, 4, 6, 8, 10]\n","Flipping `3-1` to `1-3`: -2\n"]}]}]}